investigations/cava2/Fib.v
@@ -35,13 +35,11 @@ Section Var.
     fun a => (a, a)
   }}.
 
-  Definition fib_init sz := val_of (BitVec sz) (2^(N.of_nat sz)-1).
-
   Definition fibonacci {sz: nat}: Circuit (BitVec sz ** BitVec sz) [] (BitVec sz) := {{
     let/delay r1 :=
-      let r2 := delay r1 initially (fib_init sz) in
+      let r2 := delay r1 initially (2^(N.of_nat sz)-1) in
       r1 + r2
-      initially (val_of (BitVec sz) 1) in
+      initially 1 in
     r1
   }}.
 End Var.
@@ -76,7 +74,8 @@ Lemma fibonacci_step sz state input :
     let sum := (fst state + snd state) mod (2 ^ N.of_nat sz) in
     (sum, fst state, sum).
 Proof.
-  intros; cbn [step fibonacci Bv2N Vector.of_list Primitives.binary_semantics ].
+  intros.
+  cbn [step fibonacci Bv2N Vector.of_list Primitives.binary_semantics Constant Delay LetDelay cast].
   repeat (destruct_pair_let; cbn [split_absorbed_denotation combine_absorbed_denotation List.app absorb_any fst snd ]).
   reflexivity.
 Qed.
@@ -145,4 +144,3 @@ Proof.
     autorewrite with push_length.
     erewrite <-list_unit_equiv. reflexivity. }
 Qed.
-
